PN_counter/App.fst
@@ -83,9 +83,14 @@ let rec lem_foldl (s:concrete_st) (l:log)
     |_ -> lem_foldl (do s (head l)) (tail l)
 
 //conflict resolution
-let resolve_conflict (x y:log_entry) : log =
+let resolve_conflict (x y:log_entry) : (l:log{length l > 0 /\ last l = y}) =
   cons x (cons y empty)
 
+let resolve_conflict_prop (x y:log_entry)
+  : Lemma (requires fst x <> fst y)
+          (ensures last (resolve_conflict x y) <> x)
+  = ()
+  
 // concrete merge pre-condition
 let concrete_merge_pre lca a b : prop = true
 
@@ -93,44 +98,50 @@ let concrete_merge_pre lca a b : prop = true
 let concrete_merge (lca:concrete_st) (s1:concrete_st) (s2:concrete_st{concrete_merge_pre lca s1 s2}) 
   : concrete_st = s1 + s2 - lca
 
-#push-options "--z3rlimit 50"
+#push-options "--z3rlimit 100"
 let merge_prop (lca s1 s2:st)
   : Lemma (requires is_prefix (ops_of lca) (ops_of s1) /\ 
-                    is_prefix (ops_of lca) (ops_of s2))
-          (ensures concrete_merge_pre (v_of lca) (v_of s1) (v_of s2)) = 
-  lem_foldl init_st (ops_of lca); 
+                    is_prefix (ops_of lca) (ops_of s2) /\
+                    (forall id id1. mem_id id (ops_of lca) /\ mem_id id1 (diff (ops_of s1) (ops_of lca)) ==> lt id id1) /\
+                    (forall id id1. mem_id id (ops_of lca) /\ mem_id id1 (diff (ops_of s2) (ops_of lca)) ==> lt id id1) /\
+                    (forall id. mem_id id (diff (ops_of s1) (ops_of lca)) ==> not (mem_id id (diff (ops_of s2) (ops_of lca))))) 
+          (ensures concrete_merge_pre (v_of lca) (v_of s1) (v_of s2)) =
+  lem_foldl init_st (ops_of lca);
   lem_foldl init_st (ops_of s1); 
-  lem_foldl init_st (ops_of s2)
+  lem_foldl init_st (ops_of s2);
+  split_prefix init_st (ops_of lca) (ops_of s1);
+  split_prefix init_st (ops_of lca) (ops_of s2);
+  lem_foldl (v_of lca) (diff (ops_of s1) (ops_of lca));
+  lem_foldl (v_of lca) (diff (ops_of s2) (ops_of lca))
 
-let merge_inv_s1_prop (lca s1 s2:st)
-  : Lemma (requires is_prefix (ops_of lca) (ops_of s1) /\
-                    is_prefix (ops_of lca) (ops_of s2) /\ 
-                    length (ops_of s1) > length (ops_of lca))
-          (ensures concrete_merge_pre (v_of lca) (v_of (inverse_st s1)) (v_of s2)) =
-  lem_foldl init_st (ops_of lca); 
-  lem_foldl init_st (ops_of s2); 
-  lem_foldl init_st (ops_of (inverse_st s1))
-
-let merge_inv_s2_prop (lca s1 s2:st)
+let merge_inv_prop (lca s1 s2:st)
   : Lemma (requires is_prefix (ops_of lca) (ops_of s1) /\
                     is_prefix (ops_of lca) (ops_of s2) /\
-                    length (ops_of s2) > length (ops_of lca))
-          (ensures concrete_merge_pre (v_of lca) (v_of s1) (v_of (inverse_st s2))) =
+                    Seq.length (ops_of s1) > Seq.length (ops_of lca) /\
+                    Seq.length (ops_of s2) > Seq.length (ops_of lca) /\
+                    concrete_merge_pre (v_of lca) (v_of s1) (v_of s2) /\
+                    (forall id id1. mem_id id (ops_of lca) /\ mem_id id1 (diff (ops_of s1) (ops_of lca)) ==> lt id id1) /\
+                    (forall id id1. mem_id id (ops_of lca) /\ mem_id id1 (diff (ops_of s2) (ops_of lca)) ==> lt id id1) /\
+                    (forall id. mem_id id (diff (ops_of s1) (ops_of lca)) ==> not (mem_id id (diff (ops_of s2) (ops_of lca)))))
+          (ensures (let _, last1 = un_snoc (ops_of s1) in
+                    let _, last2 = un_snoc (ops_of s2) in
+                    (last (resolve_conflict last1 last2) = last1 ==>
+                      concrete_merge_pre (v_of lca) (v_of (inverse_st s1)) (v_of s2)) /\
+                    (last (resolve_conflict last1 last2) <> last1 ==>
+                      concrete_merge_pre (v_of lca) (v_of s1) (v_of (inverse_st s2))))) =
   lem_foldl init_st (ops_of lca); 
   lem_foldl init_st (ops_of s1);
   lem_foldl init_st (ops_of (inverse_st s2))
-#pop-options
 
-#push-options "--z3rlimit 100"
 let linearizable_s1_0 (lca s1 s2:st)
-  : Lemma 
-      (requires concrete_merge_pre (v_of lca) (v_of s1) (v_of s2) /\
-                is_prefix (ops_of lca) (ops_of s1) /\
-                is_prefix (ops_of lca) (ops_of s2) /\
-                ops_of s1 = ops_of lca /\
-                foldl_prop (v_of lca) (diff (ops_of s2) (ops_of lca)))
-      (ensures concrete_merge (v_of lca) (v_of s1) (v_of s2) == 
-               seq_foldl (v_of lca) (diff (ops_of s2) (ops_of lca))) =
+  : Lemma (requires is_prefix (ops_of lca) (ops_of s1) /\
+                    is_prefix (ops_of lca) (ops_of s2) /\
+                    ops_of s1 = ops_of lca /\
+                    concrete_merge_pre (v_of lca) (v_of s1) (v_of s2) /\
+                    (forall id id1. mem_id id (ops_of lca) /\ mem_id id1 (diff (ops_of s1) (ops_of lca)) ==> lt id id1) /\
+                    (forall id id1. mem_id id (ops_of lca) /\ mem_id id1 (diff (ops_of s2) (ops_of lca)) ==> lt id id1) /\
+                    foldl_prop (v_of lca) (diff (ops_of s2) (ops_of lca)))
+          (ensures v_of s2 == concrete_merge (v_of lca) (v_of s1) (v_of s2)) =
   lem_foldl init_st (ops_of lca);
   lem_foldl init_st (ops_of s1);
   lem_foldl init_st (ops_of s2);
@@ -138,14 +149,15 @@ let linearizable_s1_0 (lca s1 s2:st)
   lem_foldl (v_of lca) (diff (ops_of s2) (ops_of lca))
 
 let linearizable_s2_0 (lca s1 s2:st)
-  : Lemma 
-      (requires concrete_merge_pre (v_of lca) (v_of s1) (v_of s2) /\
-                is_prefix (ops_of lca) (ops_of s1) /\
-                is_prefix (ops_of lca) (ops_of s2) /\
-                ops_of s2 = ops_of lca /\
-                foldl_prop (v_of lca) (diff (ops_of s1) (ops_of lca)))
-      (ensures concrete_merge (v_of lca) (v_of s1) (v_of s2) == 
-               seq_foldl (v_of lca) (diff (ops_of s1) (ops_of lca))) =
+  : Lemma (requires is_prefix (ops_of lca) (ops_of s1) /\
+                    is_prefix (ops_of lca) (ops_of s2) /\
+                    Seq.length (ops_of s1) > Seq.length (ops_of lca) /\
+                    ops_of s2 = ops_of lca /\
+                    concrete_merge_pre (v_of lca) (v_of s1) (v_of s2) /\
+                    (forall id id1. mem_id id (ops_of lca) /\ mem_id id1 (diff (ops_of s1) (ops_of lca)) ==> lt id id1) /\
+                    (forall id id1. mem_id id (ops_of lca) /\ mem_id id1 (diff (ops_of s2) (ops_of lca)) ==> lt id id1) /\
+                    foldl_prop (v_of lca) (diff (ops_of s1) (ops_of lca)))
+          (ensures v_of s1 == concrete_merge (v_of lca) (v_of s1) (v_of s2)) =
   lem_foldl init_st (ops_of lca);
   lem_foldl init_st (ops_of s1);
   lem_foldl init_st (ops_of s2);
@@ -153,40 +165,48 @@ let linearizable_s2_0 (lca s1 s2:st)
   lem_foldl (v_of lca) (diff (ops_of s1) (ops_of lca))
 
 let lem_add (lca s1 s2:int)
-  : Lemma (ensures s1 - 1 + s2 - lca + 1 = s1 + s2 - lca /\
-                   s1 + 1 + s2 - lca - 1 = s1 + s2 - lca /\
-                   s1 + (s2 - 1) - lca + 1 = s1 + s2 - lca /\
+  : Lemma (ensures s1 + (s2 - 1) - lca + 1 = s1 + s2 - lca /\
                    s1 + (s2 + 1) - lca - 1 = s1 + s2 - lca)
   = ()
-  
-let linearizable_s1_gt0 (lca s1 s2:st)
-  : Lemma 
-      (requires is_prefix (ops_of lca) (ops_of s1) /\
-                is_prefix (ops_of lca) (ops_of s2) /\
-                Seq.length (ops_of s1) > Seq.length (ops_of lca) /\
-                is_prefix (ops_of lca) (ops_of (inverse_st s1)) /\
-                concrete_merge_pre (v_of lca) (v_of s1) (v_of s2) /\
-                concrete_merge_pre (v_of lca) (v_of (inverse_st s1)) (v_of s2))
-      (ensures (let _, last1 = un_snoc (ops_of s1) in
-                concrete_do_pre (concrete_merge (v_of lca) (v_of (inverse_st s1)) (v_of s2)) last1 /\
-                concrete_merge (v_of lca) (v_of s1) (v_of s2) ==
-                do (concrete_merge (v_of lca) (v_of (inverse_st s1)) (v_of s2)) last1)) =
-  let _, last1 = un_snoc (ops_of s1) in
-  assert (concrete_do_pre (concrete_merge (v_of lca) (v_of (inverse_st s1)) (v_of s2)) last1);
+
+let linearizable_gt0 (lca s1 s2:st)
+  : Lemma (requires is_prefix (ops_of lca) (ops_of s1) /\
+                    is_prefix (ops_of lca) (ops_of s2) /\
+                    Seq.length (ops_of s1) > Seq.length (ops_of lca) /\ 
+                    Seq.length (ops_of s2) > Seq.length (ops_of lca) /\ 
+                    (let _, last1 = un_snoc (ops_of s1) in
+                     let _, last2 = un_snoc (ops_of s2) in
+                     (last (resolve_conflict last1 last2) = last1 ==>
+                           is_prefix (ops_of lca) (ops_of (inverse_st s1)) /\
+                           concrete_merge_pre (v_of lca) (v_of (inverse_st s1)) (v_of s2)) /\
+                     (last (resolve_conflict last1 last2) <> last1 ==>
+                           is_prefix (ops_of lca) (ops_of (inverse_st s2)) /\
+                           concrete_merge_pre (v_of lca) (v_of s1) (v_of (inverse_st s2)))) /\
+                    concrete_merge_pre (v_of lca) (v_of s1) (v_of s2) /\
+                    (forall id id1. mem_id id (ops_of lca) /\ mem_id id1 (diff (ops_of s1) (ops_of lca)) ==> lt id id1) /\
+                    (forall id id1. mem_id id (ops_of lca) /\ mem_id id1 (diff (ops_of s2) (ops_of lca)) ==> lt id id1) /\
+                    (forall id. mem_id id (diff (ops_of s1) (ops_of lca)) ==> not (mem_id id (diff (ops_of s2) (ops_of lca)))))
+          (ensures (let _, last1 = un_snoc (ops_of s1) in
+                    let _, last2 = un_snoc (ops_of s2) in
+                    (last (resolve_conflict last1 last2) = last1 ==>
+                      concrete_do_pre (concrete_merge (v_of lca) (v_of (inverse_st s1)) (v_of s2)) last1 /\
+                      (concrete_merge (v_of lca) (v_of s1) (v_of s2) ==
+                      do (concrete_merge (v_of lca) (v_of (inverse_st s1)) (v_of s2)) last1)) /\
+                    (last (resolve_conflict last1 last2) <> last1 ==>
+                      concrete_do_pre (concrete_merge (v_of lca) (v_of s1) (v_of (inverse_st s2))) last2 /\
+                      (concrete_merge (v_of lca) (v_of s1) (v_of s2) ==
+                      do (concrete_merge (v_of lca) (v_of s1) (v_of (inverse_st s2))) last2)))) =
+  let _,last1 = un_snoc (ops_of s1) in
+  let _,last2 = un_snoc (ops_of s2) in
+  lastop_neq (ops_of lca) (ops_of s1) (ops_of s2);
+  resolve_conflict_prop last1 last2;
+  assert (concrete_do_pre (concrete_merge (v_of lca) (v_of s1) (v_of (inverse_st s2))) last2); 
   lem_add (v_of lca) (v_of s1) (v_of s2)
 
-let linearizable_s2_gt0 (lca s1 s2:st)
-  : Lemma 
-      (requires is_prefix (ops_of lca) (ops_of s1) /\
-                is_prefix (ops_of lca) (ops_of s2) /\
-                Seq.length (ops_of s2) > Seq.length (ops_of lca) /\
-                is_prefix (ops_of lca) (ops_of (inverse_st s2)) /\
-                concrete_merge_pre (v_of lca) (v_of s1) (v_of s2) /\
-                concrete_merge_pre (v_of lca) (v_of s1) (v_of (inverse_st s2)))
-      (ensures (let _, last2 = un_snoc (ops_of s2) in
-                concrete_do_pre (concrete_merge (v_of lca) (v_of s1) (v_of (inverse_st s2))) last2 /\
-                concrete_merge (v_of lca) (v_of s1) (v_of s2) ==
-                do (concrete_merge (v_of lca) (v_of s1) (v_of (inverse_st s2))) last2)) =
-  let _, last2 = un_snoc (ops_of s2) in
-  assert (concrete_do_pre (concrete_merge (v_of lca) (v_of s1) (v_of (inverse_st s2))) last2);
-  lem_add (v_of lca) (v_of s1) (v_of s2)
+let convergence (lca s1 s2 s1':concrete_st)
+  : Lemma (requires concrete_merge_pre lca s1 s2 /\
+                    concrete_merge_pre lca s1' s2 /\
+                    concrete_merge_pre s1 (concrete_merge lca s1 s2) s1')
+          (ensures concrete_merge lca s1' s2 == concrete_merge s1 (concrete_merge lca s1 s2) s1')
+  = ()
+#pop-options
